src/ModAddSim.v
@@ -303,7 +303,7 @@ Section IMAP_OPERATIONS.
 
 End IMAP_OPERATIONS.
 
-Section ADD_RIGHT_CONG.
+Section URA_PROD.
 
   Lemma unfold_prod_add (M0 M1 : URA.t) : @URA.add (URA.prod M0 M1) = fun '(a0, a1) '(b0, b1) => (a0 ⋅ b0, a1 ⋅ b1).
   Proof. rewrite URA.unfold_add. extensionalities r0 r1. destruct r0, r1. ss. Qed.
@@ -311,17 +311,269 @@ Section ADD_RIGHT_CONG.
   Lemma unfold_prod_wf (M0 M1 : URA.t) : @URA.wf (URA.prod M0 M1) = fun r => URA.wf (fst r) /\ URA.wf (snd r).
   Proof. rewrite URA.unfold_wf. extensionalities r. destruct r. ss. Qed.
 
-  Tactic Notation "unfold_prod" :=
-    try rewrite ! unfold_prod_add;
-    rewrite unfold_prod_wf;
-    simpl.
+End URA_PROD.
 
-  Tactic Notation "unfold_prod" hyp(H) :=
-    try rewrite ! unfold_prod_add in H;
-    rewrite unfold_prod_wf in H;
-    simpl in H;
-    let H1 := fresh H in
-    destruct H as [H H1].
+Tactic Notation "unfold_prod" :=
+  try rewrite ! unfold_prod_add;
+  rewrite unfold_prod_wf;
+  simpl.
+
+Tactic Notation "unfold_prod" hyp(H) :=
+  try rewrite ! unfold_prod_add in H;
+  rewrite unfold_prod_wf in H;
+  simpl in H;
+  let H1 := fresh H in
+  destruct H as [H H1].
+
+Section ADD_RIGHT_CONG_SIM.
+
+  Context {M1 M2_src M2_tgt : Mod.t}.
+  Context {wf_src wf_tgt : WF}.
+  Context `{world : URA.t}.
+  Context (inh : inhabited wf_tgt.(T)).
+
+  Variable I : shared (state M2_src) (state M2_tgt) (ident M2_src) (ident M2_tgt) wf_src wf_tgt -> Prop.
+
+  Definition lift_ma :=
+    fun x : @shared (URA.prod threadsRA world)
+            (ModAdd M1 M2_src).(state) (ModAdd M1 M2_tgt).(state)
+            (ModAdd M1 M2_src).(ident) (ModAdd M1 M2_tgt).(ident)
+            (sum_wf wf_src wf_tgt) wf_tgt
+    => let '(ths, IM_SRC, IM_TGT, st_src, st_tgt, r) := x in
+      exists im_src0 ths_ctx0 ths_usr0,
+        let im_ctx0 := pick_ctx IM_TGT in
+        let im_tgt0 := chop_ctx inh ths_usr0 IM_TGT in
+        IM_SRC = add_ctx im_ctx0 im_src0
+        /\ NatMapP.Partition ths ths_ctx0 ths_usr0
+        /\ fst r = global_th ths_ctx0 ths_usr0
+        /\ fst st_src = fst st_tgt
+        /\ lifted I (ths_usr0, im_src0, im_tgt0, snd st_src, snd st_tgt, snd r).
+
+  Opaque lifted threadsRA URA.prod.
+
+  Lemma lift_ma_local_sim_ub R_src R_tgt (RR : R_src -> R_tgt -> Prop) ktr_src itr_tgt
+    : local_sim lift_ma RR (Vis (inl1 (inl1 Undefined)) ktr_src) itr_tgt.
+  Proof.
+    (* treat as if tid ∈ ths_ctx *)
+    intros ths IM_SRC0 IM_TGT0 st_src0 st_tgt0 [r_sha_th0 r_sha_w0] [r_ctx_th0 r_ctx_w0] INV0_0 tid ths0 THS0 VALID0_0.
+    simpl in INV0_0. des. subst r_sha_th0. unfold_prod VALID0_0.
+    exists (global_th (TIdSet.add tid ths_ctx0) ths_usr0, r_sha_w0). exists (local_th_context tid, URA.unit). splits.
+    { exists im_src0, (TIdSet.add tid ths_ctx0), ths_usr0. splits; ss.
+      eauto using NatMapP.Partition_sym, Partition_add.
+    }
+    { unfold_prod. split.
+      - eapply inv_add_new in THS0. des; subst. eapply global_th_alloc_context.
+        + eauto.
+        + eapply inv_add_new. split; ss.
+          ii. eapply THS0. eapply (Partition_In_left INV0_1). ss.
+        + ii. eapply THS0. eapply (Partition_In_right INV0_1). ss.
+      - rewrite URA.unit_id. eauto.
+    }
+    i. pfold. eapply pind9_fold. rewrite <- bind_trigger. econs.
+  Qed.
+
+  Lemma lift_ma_local_sim_ctx R (itr : itree _ R)
+    : local_sim lift_ma eq (embed_l M1 M2_src itr) (embed_l M1 M2_tgt itr).
+  Proof.
+    (* tid ∈ ths_ctx *)
+    intros ths IM_SRC0 IM_TGT0 st_src0 st_tgt0 [r_sha_th0 r_sha_w0] [r_ctx_th0 r_ctx_w0] INV0_0 tid ths0 THS0 VALID0_0.
+    simpl in INV0_0. des. subst r_sha_th0. unfold_prod VALID0_0.
+    exists (global_th (TIdSet.add tid ths_ctx0) ths_usr0, r_sha_w0), (local_th_context tid, URA.unit). splits.
+    { exists im_src0, (TIdSet.add tid ths_ctx0), ths_usr0. splits; ss.
+      eauto using NatMapP.Partition_sym, Partition_add.
+    }
+    { unfold_prod. split.
+      - eapply inv_add_new in THS0. des; subst. eapply global_th_alloc_context.
+        + eauto.
+        + eapply inv_add_new. split; ss.
+          ii. eapply THS0. eapply (Partition_In_left INV0_1). ss.
+        + ii. eapply THS0. eapply (Partition_In_right INV0_1). ss.
+      - rewrite URA.unit_id. eauto.
+    }
+    intros ths1 IM_SRC1 IM_TGT1 st_src1 st_tgt1 [r_sha_th1 r_sha_w1] [r_ctx_th1 r_ctx_w1] INV1_0 VALID1_0.
+    intros IM_TGT1' TGT fs ft.
+    simpl in INV1_0. des. subst r_sha_th1. unfold_prod VALID1_0.
+    unfold embed_l, embed_r.
+    assert (INV : lift_ma (ths1, IM_SRC1, IM_TGT1', st_src1, st_tgt1, (global_th ths_ctx1 ths_usr1, r_sha_w1))).
+    { ss. exists im_src1, ths_ctx1, ths_usr1. splits; ss.
+      - eapply pick_ctx_fair_thread in TGT. rewrite <- TGT. ss.
+      - eapply shared_rel_wf_lifted; eauto.
+        eapply chop_ctx_fair_thread1; eauto.
+        eapply local_th_context_in_context; eauto.
+    }
+    clear - INV VALID1_0 VALID1_1. move itr after tid.
+    rename
+      ths1 into ths0, ths_ctx1 into ths_ctx0, ths_usr1 into ths_usr0,
+      IM_SRC1 into IM_SRC0, IM_TGT1' into IM_TGT0, st_src1 into st_src0, st_tgt1 into st_tgt0,
+      r_sha_w1 into r_sha_w0, r_ctx_th1 into r_ctx_th0, r_ctx_w1 into r_ctx_w0,
+      INV into INV0, VALID1_0 into VALID_TH0, VALID1_1 into VALID_W0.
+    revert_until tid. ginit. gcofix CIH. i.
+    destruct_itree itr; [| | destruct e as [[|]|] ].
+    - rewrite 2 embed_state_ret, 2 map_event_ret.
+      gstep. eapply pind9_fold. econs. ss.
+      exists (NatSet.remove tid ths0), (URA.unit, URA.unit), (global_th (NatSet.remove tid ths_ctx0) ths_usr0, r_sha_w0).
+      splits; ss.
+      { unfold_prod. split.
+        - eapply global_th_dealloc_context; eauto.
+        - eauto.
+      }
+      { des. inversion INV2. subst ths_ctx1 ths_usr1. exists im_src0, (NatSet.remove tid ths_ctx0), ths_usr0. splits; ss.
+        eapply local_th_context_in_context in VALID_TH0.
+        eauto using NatMapP.Partition_sym, Partition_remove.
+      }
+    - rewrite 2 embed_state_tau, 2 map_event_tau.
+      gstep.
+      eapply pind9_fold. econs. split; ss.
+      eapply pind9_fold. econs. split; ss.
+      eapply pind9_fold. econs.
+      gfinal. left. eapply CIH; ss.
+    - rewrite 2 embed_state_vis.
+      rewrite 2 map_event_vis.
+      rewrite <- 2 bind_trigger.
+      gstep. destruct e; ss.
+      + eapply pind9_fold. eapply lsim_chooseR. i. esplit; ss.
+        eapply pind9_fold. eapply lsim_chooseL. exists x. esplit; ss.
+        eapply pind9_fold. eapply lsim_progress.
+        gfinal. left. eapply CIH; ss.
+      + eapply pind9_fold. eapply lsim_fairR. intros IM_TGT1 FAIR. esplit; ss.
+        eapply pind9_fold. eapply lsim_fairL.
+        des. inversion INV2. subst ths_ctx1 ths_usr1. exists (add_ctx (pick_ctx IM_TGT1) im_src0). split.
+        { subst. ii. destruct i; ss.
+          specialize (FAIR (inr (inl i))). unfold pick_ctx. ss. des_ifs.
+          + econs. ss.
+          + f_equal. ss.
+        }
+        split; ss.
+        eapply pind9_fold. eapply lsim_progress.
+        gfinal. left. des. eapply CIH; ss.
+        { esplits; eauto. eapply chop_ctx_fair_ctx in FAIR. rewrite <- FAIR. ss. }
+      + eapply pind9_fold. eapply lsim_observe. i.
+        gfinal. left. eapply CIH; ss.
+      + eapply pind9_fold. eapply lsim_UB.
+    - rewrite 2 embed_state_vis.
+      rewrite 2 map_event_vis. simpl.
+      rewrite <- 2 bind_trigger.
+      gstep. destruct c.
+      + eapply pind9_fold. eapply lsim_sync.
+        { eapply INV0. }
+        { instantiate (1 := (local_th_context tid, ε)). unfold_prod. split; ss. }
+        intros ths1 IM_SRC1 IM_TGT1 st_src1 st_tgt1 [r_sha_th1 r_sha_w1] [r_ctx_th1 r_ctx_w1] INV1_0 VALID1_0 IM_TGT1' TGT.
+        simpl in INV1_0. des. subst r_sha_th1. rename im_src0 into im_src1. unfold_prod VALID1_0.
+        gfinal. left. eapply CIH; ss.
+        { exists im_src1, ths_ctx1, ths_usr1. splits; ss.
+          - eapply pick_ctx_fair_thread in TGT. rewrite <- TGT. ss.
+          - eapply shared_rel_wf_lifted; eauto.
+            eapply chop_ctx_fair_thread1; eauto.
+            eapply local_th_context_in_context; eauto.
+        }
+      + eapply pind9_fold. eapply lsim_tidR. esplit; ss.
+        eapply pind9_fold. eapply lsim_tidL. esplit; ss.
+        eapply pind9_fold. eapply lsim_progress.
+        gfinal. left. eapply CIH; ss.
+    - destruct s.
+      + rewrite 2 embed_state_put. ss.
+        rewrite 2 map_event_vis. ss.
+        rewrite <- 2 bind_trigger.
+        gstep.
+        eapply pind9_fold. eapply lsim_getL. esplit; ss.
+        eapply pind9_fold. eapply lsim_getR. esplit; ss.
+        rewrite 2 map_event_vis. ss.
+        rewrite <- 2 bind_trigger.
+        eapply pind9_fold. eapply lsim_putL. esplit; ss.
+        eapply pind9_fold. eapply lsim_putR. esplit; ss.
+        eapply pind9_fold. eapply lsim_progress.
+        gfinal. left. eapply CIH; ss.
+        destruct st_src0, st_tgt0; ss. des; esplits; eauto.
+      + rewrite 2 embed_state_get. ss.
+        rewrite 2 map_event_vis. ss.
+        rewrite <- 2 bind_trigger.
+        gstep.
+        eapply pind9_fold. eapply lsim_getL. esplit; ss.
+        eapply pind9_fold. eapply lsim_getR. esplit; ss.
+        eapply pind9_fold. eapply lsim_progress.
+        des. rewrite INV3.
+        gfinal. left. eapply CIH; ss. esplits; eauto.
+  Qed.
+
+  Lemma lift_ma_local_sim_usr R_src R_tgt (RR : R_src -> R_tgt -> Prop) itr_src itr_tgt
+    (SIM : local_sim I RR itr_src itr_tgt)
+    : local_sim lift_ma RR (embed_r M1 M2_src itr_src) (embed_r M1 M2_tgt itr_tgt).
+  Proof.
+    (* tid ∈ ths_usr *)
+    eapply local_sim_clos_trans in SIM; ss.
+    intros ths IM_SRC0 IM_TGT0 st_src0 st_tgt0 [r_sha_th0 r_sha_w0] [r_ctx_th0 r_ctx_w0] INV0_0 tid ths0 THS0 VALID0_0.
+    simpl in INV0_0. des. subst r_sha_th0. unfold_prod VALID0_0.
+    move SIM at bottom.
+    assert (THS0' : TIdSet.add_new tid ths_usr0 (TIdSet.add tid ths_usr0)).
+    { eapply inv_add_new. split; ss. eapply inv_add_new in THS0. des.
+      eapply Partition_In_right in INV0_1. eauto.
+    }
+    specialize (SIM ths_usr0 im_src0 (chop_ctx inh ths_usr0 IM_TGT0) (snd st_src0) (snd st_tgt0) r_sha_w0 r_ctx_w0 INV0_4 tid (NatSet.add tid ths_usr0) THS0' VALID0_1).
+    destruct SIM as [r_sha_w1 [r_own_w1 [INV_USR [VALID_USR SIM]]]].
+    exists (global_th (NatSet.add tid ths_ctx0) ths_usr0, r_sha_w1), (local_th_user tid, r_own_w1). splits.
+    { admit. }
+    { admit. }
+    intros ths2 IM_SRC2 IM_TGT2 st_src2 st_tgt2 [r_sha_th2 r_sha_w2] [r_ctx_th2 r_ctx_w2] INV2_0 VALID2_0 IM_TGT2' TGT fs ft.
+    simpl in INV2_0. destruct INV2_0 as [im_src2 [ths_ctx2 [ths_usr2 INV2_0]]]. des. subst r_sha_th2. unfold_prod VALID2_0.
+    assert (TGT' : @fair_update _ (wf_clos_trans wf_tgt) (chop_ctx inh ths_usr2 IM_TGT2) (chop_ctx inh ths_usr2 IM_TGT2') (sum_fmap_l (tids_fmap tid ths_usr2))).
+    { eapply fair_mono with (wft_lt' := lt wf_tgt) (wft_wf' := wf wf_tgt).
+      { econs. ss. }
+      destruct wf_tgt. eapply chop_ctx_fair_thread2.
+      - eapply Partition_In_right in INV2_1. eapply INV2_1.
+      - eauto.
+    }
+    specialize (SIM ths_usr2 im_src2 (chop_ctx inh ths_usr2 IM_TGT2) (snd st_src2) (snd st_tgt2) r_sha_w2 r_ctx_w2 INV2_4 VALID2_1 (chop_ctx inh ths_usr2 IM_TGT2') TGT' fs ft).
+    unfold embed_l, embed_r.
+    assert (INV : lift_ma (ths2, IM_SRC2, IM_TGT2', st_src2, st_tgt2, (global_th ths_ctx2 ths_usr2, r_sha_w2))).
+    { admit. }
+    clear - INV VALID2_0 VALID2_1 SIM. move tid before I.
+    rename
+      ths2 into ths0, ths_ctx2 into ths_ctx0, ths_usr2 into ths_usr0,
+      im_src2 into im_src0, IM_SRC2 into IM_SRC0, IM_TGT2' into IM_TGT0, st_src2 into st_src0, st_tgt2 into st_tgt0,
+      r_sha_w2 into r_sha_w0, r_ctx_th2 into r_ctx_th0, r_ctx_w2 into r_ctx_w0, r_own_w1 into r_own_w0,
+      INV into INV0, VALID2_0 into VALID_TH0, VALID2_1 into VALID_W0.
+    revert_until tid. ginit. gcofix CIH. i. gstep. punfold SIM.
+    match type of SIM with pind9 _ _ _ _ ?RR _ _ _ _ _ ?SHA => remember RR as RR_MEM; remember SHA as SHA_MEM end.
+    revert RR ths0 ths_ctx0 ths_usr0 st_src0 st_tgt0 r_sha_w0 r_own_w0 r_ctx_th0 im_src0 IM_SRC0 IM_TGT0 INV0 VALID_TH0 VALID_W0 HeqRR_MEM HeqSHA_MEM.
+    pattern R_src, R_tgt, RR_MEM, fs, ft, r_ctx_w0, itr_src, itr_tgt, SHA_MEM.
+    revert R_src R_tgt RR_MEM fs ft r_ctx_w0 itr_src itr_tgt SHA_MEM SIM.
+    eapply pind9_acc. intros rr DEC IH R_src R_tgt RR_MEM fs ft r_ctx_w0 itr_src itr_tgt SHA_MEM. i.
+    clear DEC. subst RR_MEM SHA_MEM.
+    eapply pind9_unfold in PR; eauto with paco. eapply pind9_fold. inv PR.
+    - rewrite 2 embed_state_ret, 2 map_event_ret. econs.
+      ss. des. inversion INV2. clear INV2. subst ths_ctx1 ths_usr1 ths3 IM_SRC0.
+      exists (NatMap.remove tid ths0), (URA.unit, r_own), (global_th ths_ctx0 (NatMap.remove tid ths_usr0), r_shared2).
+      splits; ss.
+      + unfold_prod. split.
+        * eapply global_th_dealloc_user; eauto.
+        * ss.
+      + esplits; ss.
+        * eapply local_th_user_in_user in VALID_TH0.
+          eapply Partition_remove; eauto.
+        * admit.
+    - admit.
+    - admit.
+    - admit.
+    - admit.
+    - admit.
+    - admit.
+    - admit.
+    - admit.
+    - admit.
+    - admit.
+    - admit.
+    - admit.
+    - admit.
+    - admit.
+    - admit.
+    - admit.
+    - admit.
+    - admit.
+  Admitted.
+
+End ADD_RIGHT_CONG_SIM.
+
+Section ADD_RIGHT_CONG.
 
   Opaque lifted threadsRA URA.prod.
 
@@ -330,20 +582,7 @@ Section ADD_RIGHT_CONG.
     ModSim.mod_sim (ModAdd M1 M2_src) (ModAdd M1 M2_tgt).
   Proof.
     i. inv H. rename wf_tgt_inhabited into inh.
-    pose (I' := fun x : @shared (URA.prod threadsRA world)
-                       (ModAdd M1 M2_src).(state) (ModAdd M1 M2_tgt).(state)
-                       (ModAdd M1 M2_src).(ident) (ModAdd M1 M2_tgt).(ident)
-                       (sum_wf wf_src wf_tgt) wf_tgt
-                => let '(ths, IM_SRC, IM_TGT, st_src, st_tgt, r) := x in
-                  exists im_src0 ths_ctx0 ths_usr0,
-                    let im_ctx0 := pick_ctx IM_TGT in
-                    let im_tgt0 := chop_ctx inh ths_usr0 IM_TGT in
-                    IM_SRC = add_ctx im_ctx0 im_src0
-                    /\ NatMapP.Partition ths ths_ctx0 ths_usr0
-                    /\ fst r = global_th ths_ctx0 ths_usr0
-                    /\ fst st_src = fst st_tgt
-                    /\ lifted I (ths_usr0, im_src0, im_tgt0, snd st_src, snd st_tgt, snd r)
-         ).
+    pose (I' := @lift_ma M1 M2_src M2_tgt _ _ _ inh I).
     constructor 1 with _ _ _ I'; eauto.
     { clear - init.
       intro IM_TGT. specialize (init (chop_ctx inh NatSet.empty IM_TGT)).
@@ -356,182 +595,10 @@ Section ADD_RIGHT_CONG.
       - unfold_prod. split; ss. rewrite URA.unfold_wf. econs; ss. eapply Disjoint_empty.
     }
     i. specialize (funs0 fn args).
-    destruct M1 as [state1 ident1 st_init1 funs1].
-    destruct M2_src as [state2_src ident2_src st_init2_src funs2_src].
-    destruct M2_tgt as [state2_tgt ident2_tgt st_init2_tgt funs2_tgt].
-    ss. unfold add_funs. ss.
-    destruct (funs1 fn), (funs2_src fn), (funs2_tgt fn); ss.
-    - (* treat as if tid ∈ ths_ctx *)
-      intros ths IM_SRC0 IM_TGT0 st_src0 st_tgt0 [r_sha_th0 r_sha_w0] [r_ctx_th0 r_ctx_w0] INV0_0 tid ths0 THS0 VALID0_0.
-      simpl in INV0_0. des. subst r_sha_th0. unfold_prod VALID0_0.
-      exists (global_th (TIdSet.add tid ths_ctx0) ths_usr0, r_sha_w0). exists (local_th_context tid, URA.unit). splits.
-      { exists im_src0, (TIdSet.add tid ths_ctx0), ths_usr0. splits; ss.
-        eauto using NatMapP.Partition_sym, Partition_add.
-      }
-      { unfold_prod. split.
-        - eapply inv_add_new in THS0. des; subst. eapply global_th_alloc_context.
-          + eauto.
-          + eapply inv_add_new. split; ss.
-            ii. eapply THS0. eapply (Partition_In_left INV0_1). ss.
-          + ii. eapply THS0. eapply (Partition_In_right INV0_1). ss.
-        - rewrite URA.unit_id. eauto.
-      }
-      i. pfold. eapply pind9_fold. rewrite <- bind_trigger. econs.
-    - (* tid ∈ ths_ctx *)
-      intros ths IM_SRC0 IM_TGT0 st_src0 st_tgt0 [r_sha_th0 r_sha_w0] [r_ctx_th0 r_ctx_w0] INV0_0 tid ths0 THS0 VALID0_0.
-      simpl in INV0_0. des. subst r_sha_th0. unfold_prod VALID0_0.
-      exists (global_th (TIdSet.add tid ths_ctx0) ths_usr0, r_sha_w0), (local_th_context tid, URA.unit). splits.
-      { exists im_src0, (TIdSet.add tid ths_ctx0), ths_usr0. splits; ss.
-        eauto using NatMapP.Partition_sym, Partition_add.
-      }
-      { unfold_prod. split.
-        - eapply inv_add_new in THS0. des; subst. eapply global_th_alloc_context.
-          + eauto.
-          + eapply inv_add_new. split; ss.
-            ii. eapply THS0. eapply (Partition_In_left INV0_1). ss.
-          + ii. eapply THS0. eapply (Partition_In_right INV0_1). ss.
-        - rewrite URA.unit_id. eauto.
-      }
-      intros ths1 IM_SRC1 IM_TGT1 st_src1 st_tgt1 [r_sha_th1 r_sha_w1] [r_ctx_th1 r_ctx_w1] INV1_0 VALID1_0.
-      intros IM_TGT1' TGT fs ft.
-      simpl in INV1_0. des. subst r_sha_th1. unfold_prod VALID1_0.
-      unfold embed_l, embed_r. remember (k args) as itr.
-      assert (INV : I' (ths1, IM_SRC1, IM_TGT1', st_src1, st_tgt1, (global_th ths_ctx1 ths_usr1, r_sha_w1))).
-      { ss. exists im_src1, ths_ctx1, ths_usr1. splits; ss.
-        - eapply pick_ctx_fair_thread in TGT. rewrite <- TGT. ss.
-        - eapply shared_rel_wf_lifted; eauto.
-          eapply chop_ctx_fair_thread1; eauto.
-          eapply local_th_context_in_context; eauto.
-      }
-      clear - INV VALID1_0 VALID1_1.
-      rename
-        ths1 into ths0, ths_ctx1 into ths_ctx0, ths_usr1 into ths_usr0,
-        IM_SRC1 into IM_SRC0, IM_TGT1' into IM_TGT0, st_src1 into st_src0, st_tgt1 into st_tgt0,
-        r_sha_w1 into r_sha_w0, r_ctx_th1 into r_ctx_th0, r_ctx_w1 into r_ctx_w0,
-        INV into INV0, VALID1_0 into VALID_TH0, VALID1_1 into VALID_W0.
-      revert_until tid. ginit. gcofix CIH. i.
-      destruct_itree itr; [| | destruct e as [[|]|] ].
-      + rewrite 2 embed_state_ret, 2 map_event_ret.
-        gstep. eapply pind9_fold. econs. ss.
-        exists (NatSet.remove tid ths0), (URA.unit, URA.unit), (global_th (NatSet.remove tid ths_ctx0) ths_usr0, r_sha_w0).
-        splits; ss.
-        { unfold_prod. split.
-          - eapply global_th_dealloc_context; eauto.
-          - eauto.
-        }
-        { des. inversion INV2. subst ths_ctx1 ths_usr1. exists im_src0, (NatSet.remove tid ths_ctx0), ths_usr0. splits; ss.
-          eapply local_th_context_in_context in VALID_TH0.
-          eauto using NatMapP.Partition_sym, Partition_remove.
-        }
-      + rewrite 2 embed_state_tau, 2 map_event_tau.
-        gstep.
-        eapply pind9_fold. econs. split; ss.
-        eapply pind9_fold. econs. split; ss.
-        eapply pind9_fold. econs.
-        gfinal. left. eapply CIH; ss.
-      + rewrite 2 embed_state_vis.
-        rewrite 2 map_event_vis.
-        rewrite <- 2 bind_trigger.
-        gstep. destruct e; ss.
-        * eapply pind9_fold. eapply lsim_chooseR. i. esplit; ss.
-          eapply pind9_fold. eapply lsim_chooseL. exists x. esplit; ss.
-          eapply pind9_fold. eapply lsim_progress.
-          gfinal. left. eapply CIH; ss.
-        * eapply pind9_fold. eapply lsim_fairR. intros IM_TGT1 FAIR. esplit; ss.
-          eapply pind9_fold. eapply lsim_fairL.
-          des. inversion INV2. subst ths_ctx1 ths_usr1. exists (add_ctx (pick_ctx IM_TGT1) im_src0). split.
-          { subst. ii. destruct i; ss.
-            specialize (FAIR (inr (inl i))). unfold pick_ctx. ss. des_ifs.
-            + econs. ss.
-            + f_equal. ss.
-          }
-          split; ss.
-          eapply pind9_fold. eapply lsim_progress.
-          gfinal. left. des. eapply CIH; ss.
-          { esplits; eauto. eapply chop_ctx_fair_ctx in FAIR. rewrite <- FAIR. ss. }
-        * eapply pind9_fold. eapply lsim_observe. i.
-          gfinal. left. eapply CIH; ss.
-        * eapply pind9_fold. eapply lsim_UB.
-      + rewrite 2 embed_state_vis.
-        rewrite 2 map_event_vis. simpl.
-        rewrite <- 2 bind_trigger.
-        gstep. destruct c.
-        * eapply pind9_fold. eapply lsim_sync.
-          { eapply INV0. }
-          { instantiate (1 := (local_th_context tid, ε)). unfold_prod. split; ss. }
-          intros ths1 IM_SRC1 IM_TGT1 st_src1 st_tgt1 [r_sha_th1 r_sha_w1] [r_ctx_th1 r_ctx_w1] INV1_0 VALID1_0 IM_TGT1' TGT.
-          simpl in INV1_0. des. subst r_sha_th1. rename im_src0 into im_src1. unfold_prod VALID1_0.
-          gfinal. left. eapply CIH; ss.
-          { exists im_src1, ths_ctx1, ths_usr1. splits; ss.
-            - eapply pick_ctx_fair_thread in TGT. rewrite <- TGT. ss.
-            - eapply shared_rel_wf_lifted; eauto.
-              eapply chop_ctx_fair_thread1; eauto.
-              eapply local_th_context_in_context; eauto.
-          }
-        * eapply pind9_fold. eapply lsim_tidR. esplit; ss.
-          eapply pind9_fold. eapply lsim_tidL. esplit; ss.
-          eapply pind9_fold. eapply lsim_progress.
-          gfinal. left. eapply CIH; ss.
-      + destruct s.
-        * rewrite 2 embed_state_put. ss.
-          rewrite 2 map_event_vis. ss.
-          rewrite <- 2 bind_trigger.
-          gstep.
-          eapply pind9_fold. eapply lsim_getL. esplit; ss.
-          eapply pind9_fold. eapply lsim_getR. esplit; ss.
-          rewrite 2 map_event_vis. ss.
-          rewrite <- 2 bind_trigger.
-          eapply pind9_fold. eapply lsim_putL. esplit; ss.
-          eapply pind9_fold. eapply lsim_putR. esplit; ss.
-          eapply pind9_fold. eapply lsim_progress.
-          gfinal. left. eapply CIH; ss.
-          destruct st_src0, st_tgt0; ss. des; esplits; eauto.
-        * rewrite 2 embed_state_get. ss.
-          rewrite 2 map_event_vis. ss.
-          rewrite <- 2 bind_trigger.
-          gstep.
-          eapply pind9_fold. eapply lsim_getL. esplit; ss.
-          eapply pind9_fold. eapply lsim_getR. esplit; ss.
-          eapply pind9_fold. eapply lsim_progress.
-          des. rewrite INV3.
-          gfinal. left. eapply CIH; ss. esplits; eauto.
-    - (* tid ∈ ths_mod *)
-      rename funs0 into SIM.
-      eapply local_sim_clos_trans in SIM; ss.
-      intros ths IM_SRC0 IM_TGT0 st_src0 st_tgt0 [r_sha_th0 r_sha_w0] [r_ctx_th0 r_ctx_w0] INV0_0 tid ths0 THS0 VALID0_0.
-      simpl in INV0_0. des. subst r_sha_th0. unfold_prod VALID0_0.
-      move SIM at bottom.
-      assert (THS0' : TIdSet.add_new tid ths_usr0 (TIdSet.add tid ths_usr0)).
-      { eapply inv_add_new. split; ss. eapply inv_add_new in THS0. des.
-        eapply Partition_In_right in INV0_1. eauto.
-      }
-      specialize (SIM ths_usr0 im_src0 (chop_ctx inh ths_usr0 IM_TGT0) (snd st_src0) (snd st_tgt0) r_sha_w0 r_ctx_w0 INV0_4 tid (NatSet.add tid ths_usr0) THS0' VALID0_1).
-      destruct SIM as [r_sha_w1 [r_own_w1 [INV_USR [VALID_USR SIM]]]].
-      exists (global_th (NatSet.add tid ths_ctx0) ths_usr0, r_sha_w1), (local_th_user tid, r_own_w1). splits.
-      { admit. }
-      { admit. }
-      intros ths2 IM_SRC2 IM_TGT2 st_src2 st_tgt2 [r_sha_th2 r_sha_w2] [r_ctx_th2 r_ctx_w2] INV2_0 VALID2_0 IM_TGT2' TGT fs ft.
-      simpl in INV2_0. destruct INV2_0 as [im_src2 [ths_ctx2 [ths_usr2 INV2_0]]]. des. subst r_sha_th2. unfold_prod VALID2_0.
-      assert (TGT' : @fair_update _ (wf_clos_trans wf_tgt) (chop_ctx inh ths_usr2 IM_TGT2) (chop_ctx inh ths_usr2 IM_TGT2') (sum_fmap_l (tids_fmap tid ths_usr2))).
-      { eapply fair_mono with (wft_lt' := lt wf_tgt) (wft_wf' := wf wf_tgt).
-        { econs. ss. }
-        destruct wf_tgt. eapply chop_ctx_fair_thread2.
-        - eapply Partition_In_right in INV2_1. eapply INV2_1.
-        - eauto.
-      }
-      specialize (SIM ths_usr2 im_src2 (chop_ctx inh ths_usr2 IM_TGT2) (snd st_src2) (snd st_tgt2) r_sha_w2 r_ctx_w2 INV2_4 VALID2_1 (chop_ctx inh ths_usr2 IM_TGT2') TGT' fs ft).
-      unfold embed_l, embed_r. remember (k args) as itr_src. remember (k0 args) as itr_tgt.
-      assert (INV : I' (ths2, IM_SRC2, IM_TGT2', st_src2, st_tgt2, (global_th ths_ctx2 ths_usr2, r_sha_w2))).
-      { admit. }
-      clear - INV VALID2_0 VALID2_1 SIM.
-      rename
-        ths2 into ths0, ths_ctx2 into ths_ctx0, ths_usr2 into ths_usr0,
-        IM_SRC2 into IM_SRC0, IM_TGT2' into IM_TGT0, st_src2 into st_src0, st_tgt2 into st_tgt0,
-        r_sha_w2 into r_sha_w0, r_ctx_th2 into r_ctx_th0, r_ctx_w2 into r_ctx_w0, r_own_w1 into r_own_w0,
-        INV into INV0, VALID2_0 into VALID_TH0, VALID2_1 into VALID_W0.
-      revert_until tid. ginit. gcofix CIH. i. gstep.
-      punfold SIM.
-      match type of SIM with pind9 _ _ _ _ ?RR _ _ _ _ _ ?SHA => remember RR as RR_MEM; remember SHA as SHA_MEM end.
-  Admitted.
+    unfold ModAdd, add_funs; ss. des_ifs.
+    - eapply lift_ma_local_sim_ub.
+    - eapply lift_ma_local_sim_ctx.
+    - eapply lift_ma_local_sim_usr; eauto.
+  Qed.
 
 End ADD_RIGHT_CONG.
